src/ocaml/extraction/External.mli
@@ -20,6 +20,6 @@ val use_fork : bool ref
 
 val ext_all_unsat_impl : cnf list -> bool
 
-val ext_solve_imp_impl : coq_Z coq_PExpr list -> coq_Z coq_PExpr -> coq_Z coq_PExpr -> (coq_Z coq_PExpr) list * coq_Z coq_PExpr
+val ext_solve_imp_impl : coq_Z coq_PExpr list -> coq_Z coq_PExpr -> coq_Z coq_PExpr list -> (coq_Z coq_PExpr) list * (coq_Z coq_PExpr) list
 
-val ext_solve_imp_list_impl : ((coq_Z coq_PExpr list * coq_Z coq_PExpr) * coq_Z coq_PExpr) list -> ((coq_Z coq_PExpr) list * coq_Z coq_PExpr) list
+val ext_solve_imp_list_impl : ((coq_Z coq_PExpr list * coq_Z coq_PExpr) * coq_Z coq_PExpr list) list -> ((coq_Z coq_PExpr) list * (coq_Z coq_PExpr) list) list
