src/ocaml/extraction/Seqs.ml
@@ -2,16 +2,10 @@ open Eqtype
 open Seq
 open Ssrbool
 
-(** val tflatten_rec : 'a1 list -> 'a1 list list -> 'a1 list **)
-
-let rec tflatten_rec res = function
-| [] -> res
-| hd :: tl -> tflatten_rec (catrev hd res) tl
-
 (** val tflatten : 'a1 list list -> 'a1 list **)
 
 let tflatten ss =
-  tflatten_rec [] ss
+  foldl (fun r s -> catrev s r) [] ss
 
 (** val mapr_rec : ('a1 -> 'a2) -> 'a2 list -> 'a1 list -> 'a2 list **)
 
@@ -24,18 +18,25 @@ let rec mapr_rec f res = function
 let mapr f es =
   mapr_rec f [] es
 
-(** val tfilter_rec :
-    Equality.coq_type -> Equality.sort pred -> Equality.sort list ->
-    Equality.sort list -> Equality.sort list **)
-
-let rec tfilter_rec a p res = function
-| [] -> res
-| hd :: tl ->
-  if p hd then tfilter_rec a p (hd :: res) tl else tfilter_rec a p res tl
-
 (** val tfilter :
     Equality.coq_type -> Equality.sort pred -> Equality.sort list ->
     Equality.sort list **)
 
-let tfilter a p es =
-  tfilter_rec a p [] es
+let tfilter _ p es =
+  foldl (fun r x -> if p x then x :: r else r) [] es
+
+(** val zipr_rec :
+    ('a1 * 'a2) list -> 'a1 list -> 'a2 list -> ('a1 * 'a2) list **)
+
+let rec zipr_rec res_rev xs ys =
+  match xs with
+  | [] -> res_rev
+  | x :: xs0 ->
+    (match ys with
+     | [] -> res_rev
+     | y :: ys0 -> zipr_rec ((x, y) :: res_rev) xs0 ys0)
+
+(** val zipr : 'a1 list -> 'a2 list -> ('a1 * 'a2) list **)
+
+let zipr xs ys =
+  zipr_rec [] xs ys
