src/ocaml/extraction/Seqs.mli
@@ -2,18 +2,16 @@ open Eqtype
 open Seq
 open Ssrbool
 
-val tflatten_rec : 'a1 list -> 'a1 list list -> 'a1 list
-
 val tflatten : 'a1 list list -> 'a1 list
 
 val mapr_rec : ('a1 -> 'a2) -> 'a2 list -> 'a1 list -> 'a2 list
 
 val mapr : ('a1 -> 'a2) -> 'a1 list -> 'a2 list
 
-val tfilter_rec :
-  Equality.coq_type -> Equality.sort pred -> Equality.sort list ->
-  Equality.sort list -> Equality.sort list
-
 val tfilter :
   Equality.coq_type -> Equality.sort pred -> Equality.sort list ->
   Equality.sort list
+
+val zipr_rec : ('a1 * 'a2) list -> 'a1 list -> 'a2 list -> ('a1 * 'a2) list
+
+val zipr : 'a1 list -> 'a2 list -> ('a1 * 'a2) list
