src/ocaml/main/std.ml
@@ -26,7 +26,7 @@ let parse_spec file =
   let t1 = Unix.gettimeofday() in
   let _ = vprint ("Parsing Cryptoline file:\t\t") in
   try
-    let spec = spec_from_file ~vector:!use_vector_parser file in
+    let spec = spec_from_file file in
     let t2 = Unix.gettimeofday() in
     let _ = vprintln ("[OK]\t\t" ^ string_of_running_time t1 t2) in
     spec
@@ -39,7 +39,7 @@ let parse_program file =
   let t1 = Unix.gettimeofday() in
   let _ = vprint ("Parsing Cryptoline file: ") in
   try
-    let p = program_from_file ~vector:!use_vector_parser file in
+    let p = program_from_file file in
     let t2 = Unix.gettimeofday() in
     let _ = vprintln ("[OK]\t\t" ^ string_of_running_time t1 t2) in
     p
