src/ocaml/parsers/std.ml
@@ -1,12 +1,9 @@
 
 open Common
 
-let spec_from_lexbuf ?vector:(vector=false) lexbuf =
+let spec_from_lexbuf lexbuf =
   try
-    if vector then
-      VectorCryptolineParser.spec VectorCryptolineLexer.token lexbuf
-    else
-      CryptolineParser.spec CryptolineLexer.token lexbuf
+    CryptolineParser.spec CryptolineLexer.token lexbuf
   with
   | Failure msg -> raise (Failure ("Error at line " ^ string_of_int !lnum ^ ". " ^ msg))
   | Parsing.Parse_error ->
@@ -15,18 +12,15 @@ let spec_from_lexbuf ?vector:(vector=false) lexbuf =
     let msg = Printf.sprintf "Parser error at line %d char %d." l c in
     raise (Failure msg)
 
-let spec_from_file ?vector:(vector=false) file =
-  spec_from_lexbuf ~vector:vector (Lexing.from_channel (open_in file))
+let spec_from_file file =
+  spec_from_lexbuf (Lexing.from_channel (open_in file))
 
-let spec_from_string ?vector:(vector=false) str =
-  spec_from_lexbuf ~vector:vector (Lexing.from_string str)
+let spec_from_string str =
+  spec_from_lexbuf (Lexing.from_string str)
 
-let program_from_lexbuf ?vector:(vector=false) lexbuf =
+let program_from_lexbuf lexbuf =
   try
-    if vector then
-      VectorCryptolineParser.prog VectorCryptolineLexer.token lexbuf
-    else
-      CryptolineParser.prog CryptolineLexer.token lexbuf
+    CryptolineParser.prog CryptolineLexer.token lexbuf
   with
   | Failure msg -> raise (Failure ("Error at line " ^ string_of_int !lnum ^ ". " ^ msg))
   | Parsing.Parse_error ->
@@ -35,8 +29,8 @@ let program_from_lexbuf ?vector:(vector=false) lexbuf =
     let msg = Printf.sprintf "Parser error at line %d char %d." l c in
     raise (Failure msg)
 
-let program_from_file ?vector:(vector=false) file =
-  program_from_lexbuf ~vector:vector (Lexing.from_channel (open_in file))
+let program_from_file file =
+  program_from_lexbuf (Lexing.from_channel (open_in file))
 
-let program_from_string ?vector:(vector=false) str =
-  program_from_lexbuf ~vector:vector (Lexing.from_string str)
+let program_from_string str =
+  program_from_lexbuf (Lexing.from_string str)
