src/ocaml/parsers/std.mli
@@ -1,8 +1,8 @@
 
 open Ast.Cryptoline
 
-val spec_from_file : ?vector:bool -> string -> VS.t * spec
-val spec_from_string : ?vector:bool -> string -> VS.t * spec
+val spec_from_file : string -> VS.t * spec
+val spec_from_string : string -> VS.t * spec
 
-val program_from_file : ?vector:bool -> string -> program
-val program_from_string : ?vector:bool -> string -> program
+val program_from_file : string -> program
+val program_from_string : string -> program
